New (almost done) thread trace

src/ThreadTrace.v
@@ -1,3 +1,4 @@
+Require Import Lia Setoid Program.Basics.
 From hahn Require Import Hahn.
 From hahn Require Import HahnTrace.
 From hahn Require Import HahnSorted.
@@ -16,20 +17,128 @@ Notation "'E'" := (acts_set G).
 Notation "'lab'" := (lab G).
 Notation "'sb'" := (sb G).
 
+Definition thread_events (t : thread_id) : actid -> Prop := (fun e => t = tid e) ∩₁ E.
+Definition seq_set (t : thread_id) (n : nat) (x : actid) :=
+  In x (map (ThreadEvent t) (List.seq 0 n)).
+
+Hypothesis WF : Wf G.
+Hypothesis THREAD_EVENTS : forall t, exists n, thread_events t ≡₁ seq_set t n.
+
+Lemma seq_set_fin (t : thread_id) (n : nat) : set_finite (seq_set t n).
+Proof.
+  unfolder.
+  exists (map (ThreadEvent t) (List.seq 0 n)).
+  now unfold seq_set.
+Qed.
+
+Lemma all_finite (t : thread_id) : set_finite (thread_events t).
+Proof using THREAD_EVENTS.
+  destruct (THREAD_EVENTS t) as [n HEQ].
+  rewrite HEQ. apply seq_set_fin.
+Qed.
+
+Lemma seq_set_step (n : nat) (t : thread_id) :
+  seq_set t (S n) ≡₁ seq_set t n ∪₁ (eq (ThreadEvent t n)).
+Proof using.
+  unfold seq_set. rewrite seqS, map_app.
+  simpl. unfolder; splits; intros x HIN.
+  { apply in_app_iff in HIN.
+    simpl in HIN. basic_solver. }
+  apply in_app_iff.
+  destruct HIN as [HIN|HIN]; simpl; auto.
+Qed.
+
+Lemma seq_set_size (t : thread_id) (n : nat):
+  set_size (seq_set t n) = NOnum n.
+Proof using.
+  induction n.
+  { apply set_size_empty.
+    unfold seq_set. now rewrite seq0. }
+  rewrite seq_set_step.
+  replace (S n) with (n + 1) by lia.
+  apply set_size_union_disjoint; auto.
+  { apply set_size_single. }
+  admit.
+Admitted.
+
+Lemma actid_form (t : thread_id) (n : nat)
+  (LT : NOmega.lt_nat_l n (set_size (thread_events t))) :
+  E (ThreadEvent t n).
+Proof using THREAD_EVENTS.
+  eapply set_subset_inter_l.
+  { right. apply set_subset_refl2. }
+  destruct (THREAD_EVENTS t) as [N HEQ].
+  apply HEQ.
+  unfold seq_set. apply in_map.
+  apply in_seq.
+  simpl. splits; try lia.
+  now rewrite HEQ, seq_set_size in LT.
+Qed.
+
+Lemma actid_form_inv (t : thread_id) (x : actid)
+  (IN : thread_events t x) :
+  NOmega.lt_nat_l (index x) (set_size (thread_events t)).
+Proof using THREAD_EVENTS.
+  destruct (THREAD_EVENTS t) as [N HEQ].
+  apply HEQ in IN. rewrite HEQ.
+  rewrite seq_set_size. simpl.
+  unfold seq_set in IN. apply in_map_iff in IN.
+  destruct IN as [n [EQ IN]]. subst x. simpl.
+  apply in_seq in IN. lia.
+Qed.
+
+Definition thread_actid_trace (t : thread_id) : trace actid :=
+  trace_map (ThreadEvent t) (
+    match set_size (thread_events t) with
+    | NOinfinity => trace_inf (fun x => x)
+    | NOnum n => trace_fin (List.seq 0 n)
+    end
+  ).
+
+Lemma thread_actid_trace_form (t : thread_id) (n : nat)
+  (LT : NOmega.lt_nat_l n (trace_length (thread_actid_trace t))):
+  trace_nth n (thread_actid_trace t) (ThreadEvent t 0) = ThreadEvent t n.
+Proof using.
+  unfold thread_actid_trace in *.
+  destruct set_size as [ | N] in *; try easy.
+  simpl in *. rewrite map_length, seq_length in LT.
+  now rewrite map_nth, seq_nth.
+Qed.
+
+Lemma thread_actid_trace_size (t : thread_id) :
+  trace_length (thread_actid_trace t) = set_size (thread_events t).
+Proof using.
+  unfold thread_actid_trace.
+  destruct set_size as [ | n ]; try easy.
+  simpl. now rewrite length_map, seq_length.
+Qed.
+
+Lemma thread_actid_trace_correct_elemes (t : thread_id) :
+  trace_elems (thread_actid_trace t) ≡₁ thread_events t.
+Proof using.
+  unfolder.
+  splits; intros x HIN.
+  { admit. }
+  admit.
+Admitted.
+
+Lemma thread_actid_trace_correct (t : thread_id) (x y : nat)
+  (CORR : NOmega.lt_nat_l y (trace_length (thread_actid_trace t)))
+  (LT : x < y) :
+  sb (trace_nth x (thread_actid_trace t) (ThreadEvent t 0))
+     (trace_nth y (thread_actid_trace t) (ThreadEvent t 0)).
+Proof using THREAD_EVENTS.
+  assert (HLT : NOmega.lt_nat_l x
+    (trace_length
+     (thread_actid_trace t))) by (eapply NOmega.lt_lt_nat; eauto).
+  rewrite !thread_actid_trace_form by assumption.
+  unfold sb, ext_sb.
+  unfolder. splits; try easy.
+  all: try apply actid_form.
+  all: now rewrite <- thread_actid_trace_size.
+Qed.
+
 Definition thread_trace (t : thread_id) : trace label :=
-  let S := (fun e => t = tid e) ∩₁ E in
-  match excluded_middle_informative (set_finite S) with
-  | left FIN =>
-    trace_fin
-        (map (fun e => lab e)
-          (isort sb
-            (undup
-              (filterP S
-                (proj1_sig
-                    (IndefiniteDescription.constructive_indefinite_description
-                      (fun findom => forall x, S x -> In x findom)
-                      FIN))))))
-  | right _ => trace_inf (fun e => lab (ThreadEvent t e))
-  end.
+  trace_map lab (thread_actid_trace t).
 
 End ThreadTrace.
